Memory/Representation.v
@@ -1,0 +1,113 @@
+Require Import Arith ZArith Lia List Structures.Equalities Logic.FinFun.
+Require Import Vrac.Tactics Vrac.Option Vrac.Eqb Vrac.MemoryType
+  Vrac.ExecutionMemoryModel Vrac.ObservationMemoryModel
+  Vrac.Context.
+
+Module Representation(V : DecidableType)(B: Eqb.EQB)
+  (Import EMM: ExecutionMemoryModel B)
+  (Import OMM: ObservationMemoryModel B)
+  (Import Ctx: Context.CONTEXT V B EMM).
+
+  Class represents (Me: mem) (Mo : obs) := {
+      repr_valid: forall b, Me ⊨ b <-> is_valid(Mo, b) = true;
+      repr_length: forall b, Me ⊨ b -> EMM.length(Me, b) = length(Mo, b);
+      repr_isinit:
+      forall κ b δ, Me ⫢ κ @ b,δ -> (exists v, v<>Undef /\ load(κ,Me,b,δ) = ⎣v⎦)
+                              <-> is_initialized(κ, Mo, b, δ) = true
+    }.
+
+  Notation "Me '▷' Mo" :=(represents Me Mo)(at level 70).
+
+  Property presentation_access_validity:
+    forall Me Mo, Me ▷ Mo ->
+             (forall κ b δ, Me ⫢ κ @ b, δ <-> is_valid_access Mo κ b δ = true).
+  Proof.
+    intros Me Mo R κ b δ. split; intro Hva.
+    - destruct Hva as [Hv [H1 H2]].
+      unfold is_valid_access.
+      repeat destruct_and_goal.
+      + now apply R.(repr_valid).
+      + lia.
+      + rewrite <- R.(repr_length) by trivial.
+        lia.
+    - unfold is_valid_access in Hva.
+      repeat destruct_and_hyp.
+      repeat split.
+      + now apply R.(repr_valid).
+      + lia.
+      + rewrite R.(repr_length) by now apply R.(repr_valid).
+        lia.
+  Qed.
+
+  Property representation_alloc:
+    forall Me Mo, Me ▷ Mo ->
+             forall n b Me2, alloc(Me, n) = (b, Me2) ->
+                        Me2 ▷ store_block(Mo, b, n).
+  Proof.
+    intros Me Mo R n b Me2 Halloc.
+    constructor.
+    - intros b0. case_eq(B.eqb b0 b); intro Hb0.
+      + simpl_block_eqb.
+        apply valid_after_alloc_same in Halloc.
+        assert(is_valid (store_block (Mo, b, n), b) = true)
+          by (eapply storeblock_validblock_same; eauto).
+        split; auto.
+      + split; intro Hv.
+        * assert(b0<>b) by now simpl_block_eqb.
+          rewrite valid_after_alloc_other in Hv; eauto.
+          erewrite storeblock_validblock_other; eauto.
+          now apply R.(repr_valid).
+        * unfold is_valid_access in Hv; repeat destruct_and_hyp.
+          erewrite storeblock_validblock_other in Hv
+              by(try split; eauto; try simpl_block_eqb).
+          rewrite valid_after_alloc_other
+            by(try split; eauto; try simpl_block_eqb).
+          now apply R.(repr_valid).
+    - intros b0 Hv. case_eq(B.eqb b0 b); intro Hb0.
+      + simpl_block_eqb.
+        erewrite length_after_alloc_same by eauto.
+        now erewrite storeblock_length_same by eauto.
+      + assert(b0<>b) by now simpl_block_eqb.
+        erewrite length_after_alloc_other by eauto.
+        erewrite storeblock_length_other by eauto.
+        apply R.(repr_length).
+        now rewrite <- valid_after_alloc_other
+          by (try split; eauto; try simpl_block_eqb).
+    - intros κ b0 δ Hva; split; intro Hinit;
+        case_eq(B.eqb b0 b); intro Hb0.
+      + simpl_block_eqb.
+        destruct Hva as [Hv [H1 H2]].
+        assert(load (κ, Me2, b, δ) = ⎣Undef⎦)
+          by (eapply alloc_undef; repeat split; eauto;
+              now erewrite <- length_after_alloc_same by eauto).
+        destruct Hinit as [v [Hvalue Hload]].
+        assert(v = Undef) by (rewrite Hload in H; now inversion H).
+        by_contradiction.
+      + assert(b0<>b) by now simpl_block_eqb.
+        destruct Hinit as [v [Hvalue Hload]].
+        erewrite storeblock_isinit_other by eauto.
+        erewrite load_after_alloc in Hload by eauto.
+        apply R.(repr_isinit); try apply validaccess_load; eexists; eauto.
+      + simpl_block_eqb.
+        now erewrite storeblock_isinit_same in Hinit by eauto.
+      + assert(b0<>b) by now simpl_block_eqb.
+        destruct Hva as [Hv [H1 H2]].
+        erewrite length_after_alloc_other in H2 by eauto.
+        erewrite storeblock_isinit_other in Hinit by eauto.
+        erewrite load_after_alloc by eauto.
+        apply R.(repr_isinit) in Hinit; trivial.
+        repeat split; auto.
+        now erewrite <- valid_after_alloc_other by eauto.
+  Qed. 
+
+End Representation.
+        
+        
+      
+
+
+
+      
+               
+
+         
